### UN metadata for demo
### manually created

@prefix ex:     <http://example.org/> .
@prefix rdfs:   <http://www.w3.org/2000/01/rdf-schema#> .
@prefix skos:   <http://www.w3.org/2004/02/skos/core#> .
@prefix owl:    <http://www.w3.org/2002/07/owl#> .
@prefix xsd:    <http://www.w3.org/2001/XMLSchema#> .


### POPULATION ###

ex:population           a                   rdfs:Class , 
                                            owl:Class ;
                        rdfs:label          "Population"@en ;
                        skos:definition     "Total population and distribution by age and sex estimated to be consistent with the population by age and sex of the related population property"@en .

ex:census               a                   rdf:Property , 
                                            owl:ObjectProperty ;
                        rdfs:domain         ex:population ;
                        rdfs:range          xsd:gYear ;
                        rdfs:label          "Census"@en ;
                        skos:definition     "Census years property related to population"@en .

ex:officialEstimates    a                   rdf:Property , 
                                            owl:ObjectProperty ;
                        rdfs:domain         ex:population ;
                        rdfs:range          xsd:gYear ;
                        rdfs:label          "Official Estimates"@en ;
                        skos:definition     "Official estimates through years related to population"@en .

ex:deFactoPopulationAdjustment          a                   rdf:Property , 
                                                            owl:ObjectProperty ;
                                        rdfs:domain         ex:population ;
                                        rdfs:range          xsd:boolean ;
                                        rdfs:label          "Censuses"@en ;
                                        skos:definition     "Census years related to population"@en .

ex:subsequentTrends     a                   rdf:Property , 
                                            owl:ObjectProperty ;
                        rdfs:domain         ex:population ;
                        rdfs:range          xsd:boolean ;
                        rdfs:label          "Subsequent Trends"@en ;
                        skos:definition     "With estimates of the subsequent trends in fertility, mortality, and international migration"@en .

### FERTILITY ###

ex:fertility            a                   rdfs:Class , 
                                            owl:Class ;
                        rdfs:label          "Fertility"@en ;
                        skos:definition     "Total fertility rate and age pattern of fertility based on related property"@en .

ex:ageMother            a                   rdf:Property , 
                                            owl:ObjectProperty ;
                        rdfs:domain         ex:fertility ;
                        rdfs:range          xsd:gYear ;
                        rdfs:label          "Age Mother"@en ;
                        skos:definition     "Registered births classified by age of mother and the underlying female population by age through the year/years of: "@en .

ex:birthHistory         a                   rdf:Property , 
                                            owl:ObjectProperty ;
                        rdfs:domain         ex:fertility ;
                        rdfs:range          xsd:gYear ;
                        rdfs:label          "Birth-History"@en ;
                        skos:definition     "Years of birth-histories data"@en .


### CHILD MORTALITY ###

ex:childMortality       a                   rdfs:Class , 
                                            owl:Class ;
                        rdfs:label          "Child Mortality"@en ;
                        skos:definition     "Under-five mortality based on related property"@en .


### OVERALL MORTALITY ###

ex:overallMortality     ex:hasDescription   ex:overallMortalityA ,
                                            ex:overallMortalityB ,
                                            ex:overallMortalityC .




### MIGRATION ###

ex:migration            ex:hasDescription   ex:migrationA .








