### UN metadata vocaulary for demo
### manually created

@prefix ex:     <http://example.org/> .
@prefix rdfs:   <http://www.w3.org/2000/01/rdf-schema#> .
@prefix skos:   <http://www.w3.org/2004/02/skos/core#> .
@prefix owl:    <http://www.w3.org/2002/07/owl#> .
@prefix xsd:    <http://www.w3.org/2001/XMLSchema#> .


### POPULATION ###

ex:population           a                   rdfs:Class , 
                                            owl:Class ;
                        rdfs:label          "Population"@en ;
                        skos:definition     "Total population and distribution by age and sex estimated to be consistent with the population by age and sex of the related population property"@en .

ex:census               a                   rdf:Property , 
                                            owl:ObjectProperty ;
                        rdfs:domain         ex:population ;
                        rdfs:range          xsd:gYear ;
                        rdfs:label          "Census"@en ;
                        skos:definition     "Census years property related to population"@en .

ex:populationOfficialEstimates  a                   rdf:Property , 
                                                    owl:ObjectProperty ;
                                rdfs:domain         ex:population ;
                                rdfs:range          xsd:gYear ;
                                rdfs:label          "Population Official Estimates"@en ;
                                skos:definition     "Official estimates through years related to population"@en .

ex:deFactoPopulationAdjustment          a                   rdf:Property , 
                                                            owl:ObjectProperty ;
                                        rdfs:domain         ex:population ;
                                        rdfs:range          xsd:boolean ;
                                        rdfs:label          "De Facto Population Adjustment"@en ;
                                        skos:definition     "Whether or not De Facto Population Adjustment has happened"@en .

ex:subsequentTrends     a                   rdf:Property , 
                                            owl:ObjectProperty ;
                        rdfs:domain         ex:population ;
                        rdfs:range          xsd:boolean ;
                        rdfs:label          "Subsequent Trends"@en ;
                        skos:definition     "Whether or not estimates of the subsequent trends in fertility, mortality, and international migration have been considered"@en .


### FERTILITY ###

ex:fertility            a                   rdfs:Class , 
                                            owl:Class ;
                        rdfs:label          "Fertility"@en ;
                        skos:definition     "Total fertility rate and age pattern of fertility based on related property"@en .

ex:ageMother            a                   rdf:Property , 
                                            owl:ObjectProperty ;
                        rdfs:domain         ex:fertility ;
                        rdfs:range          xsd:gYear ;
                        rdfs:label          "Age Mother"@en ;
                        skos:definition     "Registered births classified by age of mother and the underlying female population by age through the year/years of: "@en .

ex:fertilityBirthHistory        a                   rdf:Property , 
                                                    owl:ObjectProperty ;
                                rdfs:domain         ex:fertility ;
                                rdfs:range          xsd:gYear ;
                                rdfs:label          "Fertility Birth-History"@en ;
                                skos:definition     "Years of birth-histories fertility data"@en .


### CHILD MORTALITY ###

ex:childMortality       a                   rdfs:Class , 
                                            owl:Class ;
                        rdfs:label          "Child Mortality"@en ;
                        skos:definition     "Under-five mortality based on related property"@en .

ex:childMortalityBirthHistory       a                   rdf:Property , 
                                                        owl:ObjectProperty ;
                                    rdfs:domain         ex:childMortality ;
                                    rdfs:range          xsd:gYear ;
                                    rdfs:label          "Child Mortality Birth-History"@en ;
                                    skos:definition     "Years of birth-histories child mortality data"@en .

ex:officialEstimateInfantChildMortality     a                   rdf:Property , 
                                                                owl:ObjectProperty ;
                                            rdfs:domain         ex:childMortality ;
                                            rdfs:range          xsd:gYear ;
                                            rdfs:label          "Official Estimates Infant and Child Mortality"@en ;
                                            skos:definition     "Years of which official estimates of infant and child mortality have been considered"@en .
           

### OVERALL MORTALITY ###

ex:overallMortality     a                   rdfs:Class , 
                                            owl:Class ;
                        rdfs:label          "Overall Mortality"@en ;
                        skos:definition     "Life expectancy at birth and age pattern of mortality based on related property"@en .

ex:overallMortalityOfficialEstimates    a                   rdf:Property , 
                                                                owl:ObjectProperty ;
                                            rdfs:domain         ex:overallMortality ;
                                            rdfs:range          xsd:gYear ;
                                            rdfs:label          "Overall Mortality Official Estimates"@en ;
                                            skos:definition     "Years of which official estimated of overall mortality have been considered"@en .

ex:adjustedForUnderregistration     a                   rdf:Property , 
                                                        owl:ObjectProperty ;
                                    rdfs:domain         ex:overallMortality ;
                                    rdfs:range          xsd:boolean ;
                                    rdfs:label          "Adjusted For Underregistration"@en ;
                                    skos:definition     "Whether or not Underregistration has been adjusted"@en .

ex:adjustedForUnderreporting        a                   rdf:Property , 
                                                        owl:ObjectProperty ;
                                    rdfs:domain         ex:overallMortality ;
                                    rdfs:range          xsd:boolean ;
                                    rdfs:label          "Adjusted For Underreporting"@en ;
                                    skos:definition     "Whether or not Underreporting of infant and child deaths has been adjusted"@en .


### MIGRATION ###

ex:migration            a                   rdfs:Class , 
                                            owl:Class ;
                        rdfs:label          "Migration"@en ;
                        skos:definition     "International migration based on related property"@en .

ex:estimatesDerivation   a                   rdf:Property , 
                                            owl:ObjectProperty ;
                        rdfs:domain         ex:migration ;
                        rdfs:range          xsd:boolean ;
                        rdfs:label          "Estimates Derivation"@en ;
                        skos:definition     "Whether or not Estimates have been derived as the differences between overall population growth and natural increase"@en .

